Improve testcase

Test/pruning/basic.bpl
@@ -1,23 +1,29 @@
-// RUN: %parallel-boogie /prune:2 "%s" > "%t"
+// RUN: %parallel-boogie /prune:2 /errorTrace:0 "%s" > "%t"
 // RUN: %diff "%s.expect" "%t"
 
-type Ty;
-const unique TBool : Ty;
-
-type TyTag;
-function Tag(Ty) : TyTag;
-
-const unique TagBool : TyTag uses {
-    axiom Tag(TBool) == TagBool;
+const unique four : int;
+const unique ProducerConst : bool uses {
+    axiom four == 4;
 }
 
-function Magic<T>(x: T): T uses {
-    axiom (forall<T> x: T :: Magic(x) == 3);
+function ConsumerFunc(x: int): int;
+
+function ProducerFunc(x: int): bool uses {
+    axiom (forall x: int :: ConsumerFunc(x) == 3);
 }
 
-procedure test() 
-  ensures Magic(4) == 3;
-  ensures TagBool == Tag(TBool);
+procedure hasAxioms()
+  requires ProducerFunc(2);
+  requires ProducerConst;
+  ensures ConsumerFunc(4) == 3;
+  ensures four == 4;
+{
+  
+}
+
+procedure doesNotHaveAxioms() 
+  ensures ConsumerFunc(4) == 3; // The ConsumerFunc axiom is pruned away, so this fails to verify
+  ensures four == 4; // The ProducerConstant axiom is pruned away, so this fails to verify 
 {
   
 }
